\documentclass[a4paper]{article}
\title{Strong Factorial Conjecture}


% ---------------------------------------------------------------------
% P A C K A G E S
% ---------------------------------------------------------------------

% typography and formatting
\usepackage[english]{babel}
\usepackage[utf8]{inputenc}
\usepackage{geometry}
\usepackage{exsheets}
\usepackage{environ}
\usepackage{graphicx}
\usepackage{cutwin}
\usepackage{pifont}

% mathematics
\usepackage{xfrac}  
\usepackage{amsthm} % for theorems, and definitions
\usepackage{amssymb}
\usepackage{amsmath}
\usepackage{textcomp}
\usepackage{mathtools}
\usepackage{mleftright} % for scaling mid bar in sets
% \usepackage{MnSymbol} % for \cupdot

% extra
\usepackage{xcolor}
\usepackage{tikz}

% ---------------------------------------------------------------------
% S E T T I N G
% ---------------------------------------------------------------------

%maybe delete later, for colorbox
\usepackage{tcolorbox}
\newtcolorbox{defbox}{colback=blue!5!white,colframe=blue!75!black}
\newtcolorbox{defboxlight}{colback=cyan!5!white,colframe=cyan!75!black}
\newtcolorbox{thmbox}{colback=orange!5!white,colframe=orange!75!black}
\newtcolorbox{rembox}{colback=purple!5!white,colframe=purple!75!black}
\newtcolorbox{exmbox}{colback=gray!5!white,colframe=gray!75!black}
\newtcolorbox{intbox}{colback=violet!5!white,colframe=violet!75!black}

% typography and formatting
\geometry{margin=3cm}

\SetupExSheets{
  counter-format = ch.qu,
  counter-within = chapter,
  question/print = true,
  solution/print = true,
}

% mathematics
\newcounter{global}

\theoremstyle{definition}
\newtheorem{definition}{Definition}[]
\newtheorem{example}{Example}[definition]

\newtheorem{theorem}[definition]{Theorem}
\newtheorem{corollary}{Corollary}
\newtheorem{lemma}[definition]{Lemma}
\newtheorem{proposition}[definition]{Proposition}

\newtheorem*{remark}{Remark}
\newtheorem*{intuition}{Intuition}

% extra
\definecolor{mathif}{HTML}{0000A0} % for conditions
\definecolor{maththen}{HTML}{CC5500} % for consequences
\definecolor{mathrem}{HTML}{8b008b} % for notes
\definecolor{mathobj}{HTML}{008800}

\usetikzlibrary{positioning}
\usetikzlibrary{shapes.geometric, arrows}

% ---------------------------------------------------------------------
% C O M M A N D S
% ---------------------------------------------------------------------

\newcommand{\norm}[1]{\left\lVert#1\right\rVert}
\newcommand{\rank}{\text{rank}}
\newcommand{\Vol}{\text{Vol}}

\newcommand{\set}[1]{\mleft\{\, #1 \,\mright\}}
\newcommand{\makeset}[2]{\mleft\{\, #1 \; \middle| \; #2 \,\mright\}}

\newcommand*\diff{\mathop{}\!\mathrm{d}}
\newcommand*\Diff{\mathop{}\!\mathrm{D}}

\newcommand\restr[2]{{% we make the whole thing an ordinary symbol
  \left.\kern-\nulldelimiterspace % automatically resize the bar with \right
  #1 % the function
  \vphantom{\big|} % pretend it's a little taller at normal size
  \right|_{#2} % this is the delimiter
  }}

% ---------------------------------------------------------------------
% R E N D E R
% ---------------------------------------------------------------------

\newif\ifshowproof
\showprooftrue

\NewEnviron{Proof}{%
    \ifshowproof%
        \begin{proof}%
            \BODY
        \end{proof}%
    \fi%
}%

\begin{document}
% \maketitle
\tableofcontents

My notes on "The Strong Factorial Conjecture" by Eric Edo and Arno van den Essen.

See: https://arxiv.org/abs/1304.3956

\section{Factorial Conjecture}
%
For the first half of the coin, the Factorial Conjecture, presented here, let \(m \in \mathbb{N}_+\) be a positive integer and consider the set of all polynomials \(\mathbb{C}[X_1, X_2, \ldots, X_m]\) in \(m\) variables over \(\mathbb{C}\). In the interest of brevity, we will denote this set by \(\mathbb{C}^{[m]} := \mathbb{C}[X_1, X_2, \ldots, X_m]\).

Equipped with the usual addition and multiplication, \(\mathbb{C}^{[m]}\) forms a \(\mathbb{C}\)-algebra, and as such, it is generated by the following monomial basis
%
\begin{align*}
    \mathcal{B} = \makeset{X_1^{l_1} \cdots X_m^{l_m}}{l_k \in \mathbb{N}_0 \text{ for all } 1 \leq k \leq m} \text{.}
\end{align*}
%
Thus, any linear map is fully specified by its values on the elements of this basis. Such linear map is the factorial map.
%
\begin{definition}[Definition 2.1]
    A factorial map is a linear map linear map \(\mathcal{L}: \mathbb{C}^{[m]} \longrightarrow \mathbb{C}\) defined by
    \begin{align*}
        \mathcal{L}(X_1^{l_1} \cdots X_m^{l_m}) = l_1! \cdots l_m! \qquad \text{ for all } l_1, \ldots, l_m \in \mathbb{N}
    \end{align*}
\end{definition}
%
\begin{example}
    Consider \(f(X) = 3X - 5XY + 7Y^2 \in \mathbb{C}^{[2]}\). Applying the factorial map yields
    \begin{align*}
        \mathcal{L}(f(X)) &= 3\mathcal{L}(X) - 5 \mathcal{L}(XY) + 7 \mathcal{L}(Y^2) \\
        &= 3 \cdot 1 - 5 \cdot 1 + 7 \cdot 2 \\
        &= 12 \text{.}
    \end{align*}
\end{example}
%
\begin{example}
    If we limit our selves to a polynomial in one indeterminate, such as \(f(X) = \sum_{k = 0}^n a_k X^k \in \mathbb{C}[X]\) for a fixed \(n \in \mathbb{N}_0\) and \(a_k \in \mathbb{C}\) for all \(1 \leq k \leq n\), we have
    \begin{align*}
        \mathcal{L}(f(X)) = \sum_{k = 0}^n a_k \mathcal{L}(X^k) = \sum_{k=0}^n a_k k!
    \end{align*}
\end{example}
%
\begin{remark}[Remark 2.2]
    Let \(\sigma \in S_n\) be a permutation on the set \(\{X_1, \ldots, X_m\}\). We extend \(\sigma\) to an automorphism \(\tilde{\sigma}\) of the \(\mathbb{C}\)-algebra \(\mathbb{C}^{[m]}\) by setting
    \begin{align*}
        \tilde{\sigma} \left( X_1^{l_1} \cdots X_m^{l_m} \right) = \sigma(X_1)^{l_1} \cdots \sigma(X_m)^{l_m} \text{.}
    \end{align*}
    Then, \(\mathcal{L}(\tilde{\sigma}(f)) = \mathcal{L}(f)\) for any \(f \in \mathbb{C}^{[m]}\).
\end{remark}
\begin{proof}
    Let \(\sigma\) also denote the permutation on \(\{1, \ldots, m\}\) where \(\sigma(X_i) = X_{\sigma(i)}\). For any monomial \(X_1^{l_1} \cdots X_m^{l_m}\), we have
    \begin{align*}
        \mathcal{L}\left(\tilde{\sigma}\left(X_1^{l_1} \cdots X_m^{l_m}\right)\right) = 
        \mathcal{L} \left(X_{\sigma(1)}^{l_1} \cdots X_{\sigma(m)}^{l_m}\right) =
        l_1 ! \cdots l_m! 
    \end{align*}
    Thus, for any monomial basis element \(B \in \mathcal{B}\), \(\mathcal{L}(\tilde{\sigma}(B)) = \mathcal{L}(B)\). By linearity of both \(\tilde{\sigma}\) and \(\mathcal{L}\), it is
    \begin{align*}
        \mathcal{L}(\tilde{\sigma}(f)) = \mathcal{L}(f) \text{ for all } f \in \mathbb{C}^{[m]} \text{.}
    \end{align*}
\end{proof}
%
\begin{remark}[Remark 2.3]
    In general, the factorial map \(\mathcal{L}\) does not preserve multiplication. However, if two polynomials \(f\) and \(g\) do not share any indeterminates, i.e. there exsists a subset \(I \subset \{1, 2, \ldots, m\}\) such that
    \begin{align*}
        f(X) \in \mathbb{C}[X_k : k \in I] \; \text{ and } \; g(X) \in \mathbb{C}[X_k : k \not\in I] \text{,}
    \end{align*}
    then indeed \(\mathcal{L}(fg) = \mathcal{L}(f)\mathcal{L}(g)\).
\end{remark}
%
\begin{proof}
    % #WIP: Can be written better ...
    Let \(B_1 \in \mathcal{B}\) and \(B_2 \in \mathcal{B}\) two monomial basis elements of \(\mathbb{C}^{[m]}\) that do not share any indeterminates, i.e. there is a subset \(I \subset \{1, 2, \ldots, m\}\) such that \(B_1 \in \mathbb{C}[X_k : k \in I]\) and \(B_2 \in \mathbb{C}[X_k : k \not\in I]\).
    
    We first want to renumber the indeterminates conveniently. Let \(\sigma\) be a permutation on \(\set{X_1, \ldots, X_m}\) and \(\tilde{\sigma}\) an extension of \(\sigma\) to an automorphism on \(\mathbb{C}^{[m]}\) such that for an \(n \in \mathbb{N}\)
    \begin{align*}
        \tilde{\sigma}(B_1) \in \mathbb{C}[X_k : k \in \{1, \ldots, n\}] \; \text{ and } \; \tilde{\sigma}(B_2) \in \mathbb{C}[X_k : k \in \{n + 1, \ldots, m\}]
    \end{align*}
    
    Now, we have
    \begin{align*}
        \mathcal{L}(B_1)\mathcal{L}(B_2) &= \mathcal{L}(\tilde{\sigma}(B_1))\mathcal{L}(\tilde{\sigma}(B_1)) \\
        &= \mathcal{L}(X_1^{l_1} \cdots X_n^{l_n})\mathcal{L}(X_{n+1}^{l_{n+1}} \cdots X_m^{l_m}) \\
        &= l_1 ! \cdots l_n ! l_{n+1}! \cdots l_m \\
        &= \mathcal{L} (B_1 B_2) \text{.}
    \end{align*}
\end{proof}
%
\begin{example}
    To illustrate that the factorial map \(\mathcal{L}\) is not compatible with the multiplication, simply consider \(f(X) = X\) and \(g(X) = X\) in \(\mathbb{C}^{[1]}\). It is
    \begin{align*}
        \mathcal{L}(fg) = \mathcal{L}(X^2) = 2 \;\text{ while } \;\mathcal{L}(f) \mathcal{L}(g) = 1 \cdot 1 = 1 \text{.}
    \end{align*}
\end{example}
%
\begin{theorem}[Conjecture 2.4]
    If \(f \in \mathbb{C}^{[m]}\) is a polynomial with \(\mathcal{L}(f^k) = 0\) for all \(k \in \mathbb{N}_+\), then \(f = 0\).
\end{theorem}
%
\begin{example}
    % I'm not sure about this example
    Consider \(f(X) = a_0 + a_1X \in \mathbb{C}^{[1]}\). For \(f\) and \(f^2\), the factorial map gives
    \begin{align*}
        \mathcal{L}(f) &= a_0 + a_1 \\
        \mathcal{L}(f^2) &= \mathcal{L}(a_0^2 + 2a_0 a_1 X + a_1^2 X^2) = a_0^2 + 2 a_0 a_1 + 2 a_1^2 \text{.}
    \end{align*}    
    If \(f\) fulfills the condition for the aforementioned conjecture, we have \(a_0 + a_1 = 0\), so \(a_0 = -a_1\) in the first equation. Substituting in the second equation, yields \(a_0^2 - 2 a_0^2 + 2a_0^2 = a_0^2 = 0\), hence \(a_0 = a_1 = 0\).
\end{example}
%
We introduce the following notation. For a polynomial \(f \in \mathbb{C}^{[m]}\), \(\mathcal{N}(f)\) denotes the number of nonzero monomials in \(f\). For example, \(\mathcal{N}(1 + X + X^2) = 3\) and \(\mathcal{N}(XYZ) = 1\).
%
\begin{definition}
    Set the following subsets of \(\mathbb{C}^{[m]}\) to be
    \begin{align*}
        F^{[m]} &= \{0\} \cup \makeset{f \in \mathbb{C}^{[m]} \setminus \{0\}}{\text{there is some }k \in \mathbb{N}_+ \text{ such that }\mathcal{L}(f^k) \neq 0} \\
        F_n^{[m]} &= \{0\} \cup \makeset{f \in \mathbb{C}^{[m]} \setminus \{0\}}{\text{there is some }k \in \{n, \ldots, n + \mathcal{N}(f) - 1\} \text{ such that } \mathcal{L}(f^k) \neq 0} \\
        F_\cap^{[m]} &= \bigcap_{n \in \mathbb{N}_+} F_n^{[m]}
    \end{align*}
    We call \(F^{[m]}\) to be the factorial set and \(F^{[m]}_\cap\) to be the strong factorial set.
\end{definition}
%
\begin{remark}
    The polynomials of the factorial set \(F^{[m]}\) are precisely the polynomials that satisfy the factorial conjecture. Thus, the factorial conjecture can be reformulated to \(F^{[m]} = \mathbb{C}^{[m]}\).
\end{remark}
%
\begin{proof}
    The contraposition of the factorial conjecture states: If \(f \neq 0\), then there is some \(k \in \mathbb{N}_+\) such that \(\mathcal{L}(f^k) \neq 0\). Thus, if the factorial conjecture is true, then \(F^{[m]} = \mathbb{C}^{[m]}\).
\end{proof}
%
\begin{theorem}[Conjecture 2.8]
    All polynomials are in the strong factorial set, i.e. \(F_\cap^{[m]} = \mathbb{C}^{[m]}\).
\end{theorem}
%
\begin{remark}
    Let \(n \in \mathbb{N}_+\) be a positive integer.
    \begin{enumerate}
        \item Let \(f \in \mathbb{C}^{[m]}\) be a polynomial. \(f \in F_n^{[m]}\) if and only if for all \(k \in \{n, \ldots, n + \mathcal{N}(f) - 1\}\)
        \begin{align*}
            \mathcal{L}(f^k) = 0 \text{ implies } f = 0 \text{.}
        \end{align*}
        \item regular system of parameters
    \end{enumerate}
\end{remark}
%
\begin{remark}
    If \(\mathcal{N}(f) = 1\), i.e. \(f\) is a monomial, then \(f \in F_\cap^{[m]}\).
\end{remark}
\begin{proof}
    If \(\mathcal{N}(f) = 1\), then \(f = X_1^{l_1} \cdots X_m^{l_m}\) and \(f^k = X_1^{l_1 k} \cdots X_m^{l_m k}\). Thus, the only case where \(\mathcal{L}(f^k) = 0\) for any \(k \in \mathbb{N}_+\) is when \(f = 0\). Hence \(f\) lies in \(F_n^{[m]}\) for all \(n \in \mathbb{N}_+\) and we have \(f \in F_\cap^{[m]}\).
\end{proof}
\begin{remark}
    If \(f \in \mathbb{R}^{[m]}_{\geq 0}\), i.e. all nonzero coefficients are real and positive, then \(f \in F_\cap^{[m]}\).
\end{remark}
\begin{proof}
    Should be straight forward.
\end{proof}
%
\begin{remark}[2.11]
    See proof in other paper.
\end{remark}
%
\begin{example}
    Consider \(f = X_1 - X_2 \in \mathbb{C}^{[2]}\). For all \(n \in \mathbb{N}_+\),
    \begin{align*}
        \mathcal{L}(f^n) = \mathcal{L} \left( \sum_{k = 0}^n \binom{n}{k} X_1^{n-k}(-X_2)^k \right) = \sum_{k=0}^n \binom{n}{k} (n-k)! k! (-1)^k = \sum_{k=0}^n \frac{n!}{k!} k! (-1)^k = n! \sum_{k=0}^n (-1)^k
    \end{align*}
    Hence \(\mathcal{L}(f^n) = n!\) if \(n\) is even and \(\mathcal{L}(f^n) = 0\) otherwise. Since \(n\) or \(n + 1\) is even, we have \(f \in F_n^{[2]}\). Thus \(f \in F_\cap^{[2]}\).
    % #WIP: this example shows that SFC(2) can not be true in positive characteristc ... im not quite sure why
\end{example}
\newpage
\section{Rigidity Conjecture}
\begin{definition}
    Let \(f(X) \in \mathbb{C}[[X]]\) be a power series. We call a power series \(f^{-1}(X) \in \mathbb{C}[[X]]\) the compositional inverse of \(f\), if it satisfies \(f(f^{-1}(X)) = f^{-1}(f(X)) = X\). 
\end{definition}
\begin{proposition}
    A power series \(f(X) = a_0 + a_1 X + \cdots\in \mathbb{C}[[X]]\) has a compositional inverse if and only if \(a_0 = 0\) and \(a_1 \neq 0\). Moreover, if the compositional inverse exists, then it is unique. 
\end{proposition}
\begin{proof}
    Assume \(f\) has a compositional inverse and denote the compositional inverse by \(f^{-1}(X) = b_0 + b_1 X + b_2 X^2 + \cdots\). Writing out \(f(f^{-1}(X)) = X\) gives
    \begin{align*}
        a_0 + a_1 (b_0 + b_1 X + b_2 X^2 + \cdots)
    \end{align*}
\end{proof}

\subsection{Rigidity Conjecture}
%
\begin{theorem}[Conjecture 2.13]
    Let \(a(X) \in \mathbb{C}[X]\) be a polynomial of degree less or equal to \(m + 1 \in \mathbb{N}_+\) such that \(a(X) \equiv X \mod{X^2}\). If \(m\) consecutive coefficient of the compositional inverse \(a^{-1}(X)\) vanish, i.e. \(b_{n+1} = b_{n+2} = \cdots = b_{n+m} = 0\) for some \(n \in \mathbb{N}_+\) then \(a(X) = X\).
\end{theorem}
%
\begin{remark}
    If we denote the polynomial \(a(X)\) by \(\sum_{k \in \mathbb{N}_0}a_k X^k\) for some \(a_k \in \mathbb{C}\) for all \(k \in \mathbb{N}_0\), then the condition \(a(X) \equiv X \mod{X^2}\) amounts to \(a_0 = 0\) and \(a_1 = 1\). #UNSURE, BUT PRETTY SURE WE HAVE THIS CONDITION TO ENSURE THE INVERSE EVEN EXISTS.
\end{remark}
%
\begin{theorem}[Conjecture 2.14]
    Let \(a(X) \in \mathbb{C}[X]\) be a polynomial of degree less or equal to \(m + 1 \in \mathbb{N}_+\) such that \(a(X) \equiv X \mod{X^2}\). If the coefficients of \(X^{n+1}, \ldots, X^{n+m}\) of the compositional inverse vanish, then \(a(X) = X\).
\end{theorem}
%
\begin{remark}
    \(R(m)\) if and only if \(R(m)_n\) for all \(n \in \mathbb{N}_+\).
\end{remark}
%
% copied from Edo & van den Essen
\begin{lemma}[Lemma 2.16]
    Let \(f \in \mathbb{C}[[X]]\) and \(g \in \mathbb{C}[[X]]\) be two formal series such that \(f(X) \equiv g(X) \mod{X^2}\), i.e. the constant and the coefficient of the first degree agree. If \(f(X) \equiv g(X) \mod{X^n}\) for some integer \(n \geq 2\) then \(f^{-1}(X) \equiv g^{-1}(X) \mod{X^n}\).
\end{lemma}
\begin{proof}
    % TODO:
\end{proof}
%
\begin{proposition}
    \begin{enumerate}
        \item The polynomial \(a(X)\) is invertible for the composition.
        \item For all \(i \in \set{1, \ldots, \text{deg}(a - 1)}\), the coefficient \(a_i\) is nilpotent element in \(A\).
              I just don't see this ...
    \end{enumerate}
\end{proposition}
%
The following lemma and proof are due to \#XXX.
%
\begin{example}[See 5.4.4]
    \(f(X) = X e^{-X} = X \sum_{k=0}^\infty \frac{(-1)^k}{k!} X^k\)
    \begin{align*}
        [X^n]f^{-1}(X) = \frac{1}{n} [X^{n-1}] e^{nX}
    \end{align*}
\end{example}


\begin{lemma}[Lemma 2.20 (Additive Inversion Formula)]
    Let \(\alpha_1, \ldots, \alpha_m \in \mathbb{C}\) be complex numbers. The formal inverse of \(a(X) = X(1 - (\alpha_1 X + \cdots + \alpha_m X^m))\) is given by the following formula
    \begin{align*}
        a^{-1}(X) & = X \mleft( 1 + \frac{1}{n + 1} \sum_{n \geq 1} u_n X^n \mright)
        \intertext{where}
        u_n       & = \frac{1}{n!} \sum_{j_1 + 2 j_2 + \cdots + m j_m = n} \frac{(n + j_1 + \cdots + j_m)!}{j_1 ! \cdots j_m!} \alpha_1^{j_1} \cdots \alpha_m^{j_m}
    \end{align*}
\end{lemma}

\begin{proposition}[Proposition 2.23]
    Let \(\alpha_1, \ldots, \alpha_m \in \mathbb{C}\) be complex numbers and let \((u_n)_{n \in \mathbb{N}_+}\) be a sequence defined by AIF in Lemma 2.20. For all \(n \in \mathbb{N}_+\), the Rigidity Conjecture \(R(m)_n\) is equivalent to the following implication: If \(u_n = \cdots = u_{n + m - 1} = 0\) then \(\alpha_1 = \cdots = \alpha_m = 0\).
\end{proposition}

\begin{proof}

\end{proof}

\begin{theorem}
    \begin{enumerate}
        \item The inclusion \(E^{[m]} \subset F_n^{[m]}\) implies \(R(m)_n\)
    \end{enumerate}
\end{theorem}

\begin{definition}
    \begin{align*}
        E^{[m]}   & = \makeset{X_1 \cdots X_m (\mu_1 X_1 + \cdots + \mu_m X_m)}{\mu_1, \ldots, \mu_m \in \mathbb{C}} \subset                                  \\
        F^{[m]}_n & = \makeset{f \in \mathbb{C}^{[m]} \setminus \{0\}}{\mathcal{L}(f^k) \neq 0 \text{ for some } n \leq k \leq \mathcal{N}(f) - 1} \cup \{0\}
    \end{align*}
\end{definition}

\end{document}